MirrorCharge!/src/MirrorCharge/Java/Cancelation.v
@@ -1,4 +1,5 @@
 Require Import MirrorCore.Lambda.Expr.
+
 Require Import MirrorCore.STac.STac.
 Require MirrorCore.syms.SymEnv.
 Require MirrorCore.syms.SymSum.
@@ -21,31 +22,29 @@ Local Existing Instance RSym_ilfunc.
 Local Existing Instance RS.
 Local Existing Instance Expr_expr.
 
-Local Notation "a @ b" := (@App typ _ a b) (at level 30).
-Local Notation "\ t -> e" := (@Abs typ _ t e) (at level 40).
-
+(** NOTE: this is for [locals -> HProp] **)
 Definition sls : SepLogFoldEx.SepLogSpec typ func :=
 {| SepLogFoldEx.is_pure := fun (e : expr typ func) =>
                 match e with
-                  | Inj (inr (ilf_true _))
-                  | Inj (inr (ilf_false _)) => true
+                  | mTrue [_]
+                  | mFalse [_] => true
                   | App (App (Inj (inl (inr (pAp _ _)))) (App (Inj (inl (inr (pConst _)))) (Inj (inr (ilf_embed tyProp _))))) _ => true
                   | _ => false
                 end
  ; SepLogFoldEx.is_emp := fun e => false
  ; SepLogFoldEx.is_star := fun (e : expr typ func) =>
                 match e with
-                  | Inj (inl (inr (pStar _))) => true
+                  | mfStar [_] => true
                   | _ => false
                 end
  ; SepLogFoldEx.is_and := fun (e : expr typ func) =>
                 match e with
-                  | Inj (inr (ilf_and _)) => true
+                  | mfAnd [_] => true
                   | _ => false
                 end
  ; SepLogFoldEx.is_ex := fun (e : expr typ func) =>
                 match e with
-                  | Inj (inr (ilf_exists t u)) => Some t
+                  | mfExists [t, _] => Some t
                   | _ => None
                 end
  |}.
@@ -96,21 +95,23 @@ Let doUnifySepLog (tus tvs : EnvI.tenv typ) (s : CascadeSubst subst subst) (e1 e
 
 Let ssl : SynSepLog typ func :=
 {| e_star := fun l r =>
+               let nested_match := match r with
+		                           | mEmp [_] => l
+		                           | _ => mkStar tySasn l r
+		                           end in
                match l with
-                 | Inj (inl (inr (pEmp _))) => r
-                 | _ => match r with
-                          | Inj (inl (inr (pEmp _))) => l
-                          | _ => mkStar tySasn l r
-                        end
+                 | mEmp [_] => r
+                 | _ => nested_match
                end
  ; e_emp := mkEmp tySasn
  ; e_and := fun l r =>
+ 			  let nested_match := match r with
+		                          | mTrue [_] => l
+		                          | _ => mkAnd tySasn l r
+		                          end in
               match l with
-                | Inj (inr (ilf_true _)) => r
-                | _ => match r with
-                         | Inj (inr (ilf_true _)) => l
-                         | _ => mkAnd tySasn l r
-                       end
+                | mEmp [_] => r
+                | _ => nested_match
               end
  ; e_true := mkTrue tySasn
  |}.
@@ -118,7 +119,7 @@ Let ssl : SynSepLog typ func :=
 Definition eproveTrue (s : CascadeSubst subst subst) (e : expr typ func)
 : option (CascadeSubst subst subst) :=
   match e with
-    | Inj (inr (ilf_true _)) => Some s
+    | mTrue [_] => Some s
     | _ => None
   end.
 
@@ -202,13 +203,10 @@ Definition the_canceller tus tvs (lhs rhs : expr typ func)
 Definition stac_cancel : stac typ (expr typ func) subst :=
   fun tus tvs s hyps e =>
     match e with
-      | App (App (Inj (inr (ilf_entails tySasn))) L) R =>
+      | mEntails [tySasn, L, R] =>
         match the_canceller tus tvs L R s with
           | inl (l,r,s') =>
-            let e' :=
-                mkEntails tySasn l r
-            in
-            More tus tvs s hyps e'
+            More tus tvs s hyps (mkEntails tySasn l r)
           | inr s' => @Solved _ _ _ nil nil s'
         end
       | _ => More nil nil s hyps e
